Exercise 5.3
============

Let :math:`\boldsymbol{x}, \boldsymbol{y} \in \mathbb{R}^2, k \in \mathbb{R}`.
We will write :math:`x_1` for the first component of :math:`\boldsymbol{x}`,
:math:`x_2` for the second component of :math:`\boldsymbol{x}`, and so on.

Then:

.. math::
  k (\boldsymbol{x} + \boldsymbol{y})
    &= k (\begin{bmatrix}x_1\\x_2\end{bmatrix} + \begin{bmatrix}y_1\\y_2\end{bmatrix}) \\
    &= k (\begin{bmatrix}x_1 + y_1\\x_2 + y_2\end{bmatrix}) \\
    &= \begin{bmatrix}k(x_1 + y_1)\\k(x_2 + y_2)\end{bmatrix} \\
    &= \begin{bmatrix}kx_1 + ky_1\\kx_2 + ky_2\end{bmatrix} \\
    &= \begin{bmatrix}kx_1\\kx_2\end{bmatrix} + \begin{bmatrix}ky_1\\ky_2\end{bmatrix} \\
    &= k \begin{bmatrix}x_1\\x_2\end{bmatrix} + k \begin{bmatrix}y_1\\y_2\end{bmatrix} \\
    &= k\boldsymbol{x} + k\boldsymbol{y}

